proof/agp32UpdateScript.sml
@@ -99,7 +99,10 @@ Theorem IF_instr_update_unchanged_state_items:
   !fext s s'.
     ((IF_instr_update fext s s').command = s'.command) /\
     ((IF_instr_update fext s s').state = s'.state) /\
-    ((IF_instr_update fext s s').R = s'.R)
+    ((IF_instr_update fext s s').R = s'.R) /\
+    ((IF_instr_update fext s s').data_addr = s'.data_addr) /\
+    ((IF_instr_update fext s s').data_wstrb = s'.data_wstrb) /\
+    ((IF_instr_update fext s s').data_wdata = s'.data_wdata)
 Proof
   rw [IF_instr_update_def]
 QED
@@ -249,7 +252,10 @@ Theorem IF_PC_input_update_unchanged_state_items:
   !fext s s'.
     ((IF_PC_input_update fext s s').command = s'.command) /\
     ((IF_PC_input_update fext s s').state = s'.state) /\
-    ((IF_PC_input_update fext s s').R = s'.R)
+    ((IF_PC_input_update fext s s').R = s'.R) /\
+    ((IF_PC_input_update fext s s').data_addr = s'.data_addr) /\
+    ((IF_PC_input_update fext s s').data_wstrb = s'.data_wstrb) /\
+    ((IF_PC_input_update fext s s').data_wdata = s'.data_wdata)
 Proof
   rw [IF_PC_input_update_def]
 QED
@@ -347,7 +353,10 @@ Theorem ID_opc_func_update_unchanged_state_items:
   !fext s s'.
     ((ID_opc_func_update fext s s').command = s'.command) /\
     ((ID_opc_func_update fext s s').state = s'.state) /\
-    ((ID_opc_func_update fext s s').R = s'.R)
+    ((ID_opc_func_update fext s s').R = s'.R) /\
+    ((ID_opc_func_update fext s s').data_addr = s'.data_addr) /\
+    ((ID_opc_func_update fext s s').data_wstrb = s'.data_wstrb) /\
+    ((ID_opc_func_update fext s s').data_wdata = s'.data_wdata)
 Proof
   rw [ID_opc_func_update_def]
 QED
@@ -453,7 +462,10 @@ Theorem ID_imm_update_unchanged_state_items:
   !fext s s'.
     ((ID_imm_update fext s s').command = s'.command) /\
     ((ID_imm_update fext s s').state = s'.state) /\
-    ((ID_imm_update fext s s').R = s'.R)
+    ((ID_imm_update fext s s').R = s'.R) /\
+    ((ID_imm_update fext s s').data_addr = s'.data_addr) /\
+    ((ID_imm_update fext s s').data_wstrb = s'.data_wstrb) /\
+    ((ID_imm_update fext s s').data_wdata = s'.data_wdata)
 Proof
   rw [ID_imm_update_def]
 QED
@@ -559,7 +571,10 @@ Theorem ID_data_update_unchanged_state_items:
   !fext s s'.
     ((ID_data_update fext s s').command = s'.command) /\
     ((ID_data_update fext s s').state = s'.state) /\
-    ((ID_data_update fext s s').R = s'.R)
+    ((ID_data_update fext s s').R = s'.R) /\
+    ((ID_data_update fext s s').data_addr = s'.data_addr) /\
+    ((ID_data_update fext s s').data_wstrb = s'.data_wstrb) /\
+    ((ID_data_update fext s s').data_wdata = s'.data_wdata)
 Proof
   rw [ID_data_update_def]
 QED
@@ -680,7 +695,10 @@ Theorem ID_data_check_update_unchanged_state_items:
   !fext s s'.
     ((ID_data_check_update fext s s').command = s'.command) /\
     ((ID_data_check_update fext s s').state = s'.state) /\
-    ((ID_data_check_update fext s s').R = s'.R)
+    ((ID_data_check_update fext s s').R = s'.R) /\
+    ((ID_data_check_update fext s s').data_addr = s'.data_addr) /\
+    ((ID_data_check_update fext s s').data_wstrb = s'.data_wstrb) /\
+    ((ID_data_check_update fext s s').data_wdata = s'.data_wdata)
 Proof
   rw [ID_data_check_update_def]
 QED
@@ -816,7 +834,10 @@ Theorem EX_ALU_input_imm_update_unchanged_state_items:
   !fext s s'.
     ((EX_ALU_input_imm_update fext s s').command = s'.command) /\
     ((EX_ALU_input_imm_update fext s s').state = s'.state) /\
-    ((EX_ALU_input_imm_update fext s s').R = s'.R)
+    ((EX_ALU_input_imm_update fext s s').R = s'.R) /\
+    ((EX_ALU_input_imm_update fext s s').data_addr = s'.data_addr) /\
+    ((EX_ALU_input_imm_update fext s s').data_wstrb = s'.data_wstrb) /\
+    ((EX_ALU_input_imm_update fext s s').data_wdata = s'.data_wdata)
 Proof
   rw [EX_ALU_input_imm_update_def]
 QED
@@ -969,7 +990,10 @@ Theorem EX_ALU_update_unchanged_state_items:
   !fext s s'.
     ((EX_ALU_update fext s s').command = s'.command) /\
     ((EX_ALU_update fext s s').state = s'.state) /\
-    ((EX_ALU_update fext s s').R = s'.R)
+    ((EX_ALU_update fext s s').R = s'.R)  /\
+    ((EX_ALU_update fext s s').data_addr = s'.data_addr) /\
+    ((EX_ALU_update fext s s').data_wstrb = s'.data_wstrb) /\
+    ((EX_ALU_update fext s s').data_wdata = s'.data_wdata)
 Proof
   rw [EX_ALU_update_def] >>
   Cases_on_word_value `s'.EX.EX_func` >> fs []
@@ -1115,7 +1139,10 @@ Theorem EX_SHIFT_update_unchanged_state_items:
   !fext s s'.
     ((EX_SHIFT_update fext s s').command = s'.command) /\
     ((EX_SHIFT_update fext s s').state = s'.state) /\
-    ((EX_SHIFT_update fext s s').R = s'.R)
+    ((EX_SHIFT_update fext s s').R = s'.R) /\
+    ((EX_SHIFT_update fext s s').data_addr = s'.data_addr) /\
+    ((EX_SHIFT_update fext s s').data_wstrb = s'.data_wstrb) /\
+    ((EX_SHIFT_update fext s s').data_wdata = s'.data_wdata)
 Proof
   rw [EX_SHIFT_update_def] >>
   Cases_on_word_value `(1 >< 0) s'.EX.EX_func` >> fs []
@@ -1252,7 +1279,10 @@ Theorem EX_jump_sel_addr_update_unchanged_state_items:
   !fext s s'.
     ((EX_jump_sel_addr_update fext s s').command = s'.command) /\
     ((EX_jump_sel_addr_update fext s s').state = s'.state) /\
-    ((EX_jump_sel_addr_update fext s s').R = s'.R)
+    ((EX_jump_sel_addr_update fext s s').R = s'.R) /\
+    ((EX_jump_sel_addr_update fext s s').data_addr = s'.data_addr) /\
+    ((EX_jump_sel_addr_update fext s s').data_wstrb = s'.data_wstrb) /\
+    ((EX_jump_sel_addr_update fext s s').data_wdata = s'.data_wdata)
 Proof
   rw [EX_jump_sel_addr_update_def]
 QED
@@ -1396,7 +1426,10 @@ Theorem MEM_ctrl_update_unchanged_state_items:
   !fext s s'.
     ((MEM_ctrl_update fext s s').command = s'.command) /\
     ((MEM_ctrl_update fext s s').state = s'.state) /\
-    ((MEM_ctrl_update fext s s').R = s'.R)
+    ((MEM_ctrl_update fext s s').R = s'.R) /\
+    ((MEM_ctrl_update fext s s').data_addr = s'.data_addr) /\
+    ((MEM_ctrl_update fext s s').data_wstrb = s'.data_wstrb) /\
+    ((MEM_ctrl_update fext s s').data_wdata = s'.data_wdata)
 Proof
   rw [MEM_ctrl_update_def]
 QED
@@ -1558,7 +1591,10 @@ Theorem WB_update_unchanged_state_items:
   !fext s s'.
     ((WB_update fext s s').command = s'.command) /\
     ((WB_update fext s s').state = s'.state) /\
-    ((WB_update fext s s').R = s'.R)
+    ((WB_update fext s s').R = s'.R) /\
+    ((WB_update fext s s').data_addr = s'.data_addr) /\
+    ((WB_update fext s s').data_wstrb = s'.data_wstrb) /\
+    ((WB_update fext s s').data_wdata = s'.data_wdata)
 Proof
   rw [WB_update_def]
 QED
@@ -1712,7 +1748,10 @@ Theorem Hazard_ctrl_unchanged_state_items:
   !fext s s'.
     ((Hazard_ctrl fext s s').command = s'.command) /\
     ((Hazard_ctrl fext s s').state = s'.state) /\
-    ((Hazard_ctrl fext s s').R = s'.R)
+    ((Hazard_ctrl fext s s').R = s'.R) /\
+    ((Hazard_ctrl fext s s').data_addr = s'.data_addr) /\
+    ((Hazard_ctrl fext s s').data_wstrb = s'.data_wstrb) /\
+    ((Hazard_ctrl fext s s').data_wdata = s'.data_wdata)
 Proof
   rw [Hazard_ctrl_def]
 QED
@@ -1815,7 +1854,10 @@ Theorem Acc_compute_unchanged_state_items:
   !fext s s'.
     ((Acc_compute fext s s').command = s'.command) /\
     ((Acc_compute fext s s').state = s'.state) /\
-    ((Acc_compute fext s s').R = s'.R)
+    ((Acc_compute fext s s').R = s'.R) /\
+    ((Acc_compute fext s s').data_addr = s'.data_addr) /\
+    ((Acc_compute fext s s').data_wstrb = s'.data_wstrb) /\
+    ((Acc_compute fext s s').data_wdata = s'.data_wdata)
 Proof
   rw [Acc_compute_def]
 QED
@@ -1911,7 +1953,10 @@ Theorem IF_PC_update_unchanged_state_items:
   !fext s s'.
     ((IF_PC_update fext s s').command = s'.command) /\
     ((IF_PC_update fext s s').state = s'.state) /\
-    ((IF_PC_update fext s s').R = s'.R)
+    ((IF_PC_update fext s s').R = s'.R) /\
+    ((IF_PC_update fext s s').data_addr = s'.data_addr) /\
+    ((IF_PC_update fext s s').data_wstrb = s'.data_wstrb) /\
+    ((IF_PC_update fext s s').data_wdata = s'.data_wdata)
 Proof
   rw [IF_PC_update_def]
 QED
@@ -2008,7 +2053,10 @@ Theorem ID_pipeline_unchanged_state_items:
   !fext s s'.
     ((ID_pipeline fext s s').command = s'.command) /\
     ((ID_pipeline fext s s').state = s'.state) /\
-    ((ID_pipeline fext s s').R = s'.R)
+    ((ID_pipeline fext s s').R = s'.R) /\
+    ((ID_pipeline fext s s').data_addr = s'.data_addr) /\
+    ((ID_pipeline fext s s').data_wstrb = s'.data_wstrb) /\
+    ((ID_pipeline fext s s').data_wdata = s'.data_wdata)
 Proof
   rw [ID_pipeline_def]
 QED
@@ -2115,7 +2163,10 @@ QED
 Theorem REG_write_unchanged_state_items:
   !fext s s'.
     ((REG_write fext s s').command = s'.command) /\
-    ((REG_write fext s s').state = s'.state)
+    ((REG_write fext s s').state = s'.state) /\
+    ((REG_write fext s s').data_addr = s'.data_addr) /\
+    ((REG_write fext s s').data_wstrb = s'.data_wstrb) /\
+    ((REG_write fext s s').data_wdata = s'.data_wdata)
 Proof
   rw [REG_write_def]
 QED
@@ -2214,7 +2265,10 @@ Theorem EX_pipeline_unchanged_state_items:
   !fext s s'.
     ((EX_pipeline fext s s').command = s'.command) /\
     ((EX_pipeline fext s s').state = s'.state) /\
-    ((EX_pipeline fext s s').R = s'.R)
+    ((EX_pipeline fext s s').R = s'.R) /\
+    ((EX_pipeline fext s s').data_addr = s'.data_addr) /\
+    ((EX_pipeline fext s s').data_wstrb = s'.data_wstrb) /\
+    ((EX_pipeline fext s s').data_wdata = s'.data_wdata)
 Proof
   rw [EX_pipeline_def]
 QED
@@ -2320,7 +2374,10 @@ Theorem MEM_pipeline_unchanged_state_items:
   !fext s s'.
     ((MEM_pipeline fext s s').command = s'.command) /\
     ((MEM_pipeline fext s s').state = s'.state) /\
-    ((MEM_pipeline fext s s').R = s'.R)
+    ((MEM_pipeline fext s s').R = s'.R) /\
+    ((MEM_pipeline fext s s').data_addr = s'.data_addr) /\
+    ((MEM_pipeline fext s s').data_wstrb = s'.data_wstrb) /\
+    ((MEM_pipeline fext s s').data_wdata = s'.data_wdata)
 Proof
   rw [MEM_pipeline_def]
 QED
@@ -2435,7 +2492,10 @@ Theorem WB_pipeline_unchanged_state_items:
   !fext s s'.
     ((WB_pipeline fext s s').command = s'.command) /\
     ((WB_pipeline fext s s').state = s'.state) /\
-    ((WB_pipeline fext s s').R = s'.R)
+    ((WB_pipeline fext s s').R = s'.R) /\
+    ((WB_pipeline fext s s').data_addr = s'.data_addr) /\
+    ((WB_pipeline fext s s').data_wstrb = s'.data_wstrb) /\
+    ((WB_pipeline fext s s').data_wdata = s'.data_wdata)
 Proof
   rw [WB_pipeline_def]
 QED
@@ -3545,6 +3605,35 @@ Theorem agp32_command_state_updated_by_agp32_next_state:
     s = agp32 fext fbits t ==>
     ((agp32 fext fbits (SUC t)).command = (agp32_next_state (fext t) s s).command) /\
     ((agp32 fext fbits (SUC t)).state = (agp32_next_state (fext t) s s).state)
+Proof
+  rw [agp32_def,mk_module_def,mk_circuit_def] >>
+  qpat_abbrev_tac `s' = mk_circuit (procs _) (procs _) (agp32_init fbits) fext t` >>
+  qpat_abbrev_tac `s'' = procs _ (fext t) s' s'` >>
+  clist_update_state_tac >>
+  fs [Abbr `s13`,Abbr `s12`,Abbr `s11`,Abbr `s10`,Abbr `s9`,Abbr `s8`,Abbr `s7`,
+      Abbr `s6`,Abbr `s5`,Abbr `s4`,Abbr `s3`,Abbr `s2`,Abbr `s1`,Abbr `s''`,
+      Hazard_ctrl_unchanged_state_items,WB_update_unchanged_state_items,
+      MEM_ctrl_update_unchanged_state_items,IF_PC_input_update_unchanged_state_items,
+      EX_jump_sel_addr_update_unchanged_state_items,EX_SHIFT_update_unchanged_state_items,
+      EX_ALU_update_unchanged_state_items,EX_ALU_input_imm_update_unchanged_state_items,
+      ID_data_check_update_unchanged_state_items,
+      ID_data_update_unchanged_state_items,ID_imm_update_unchanged_state_items,
+      ID_opc_func_update_unchanged_state_items,IF_instr_update_unchanged_state_items] >>
+  slist_update_state_tac >>
+  fs [Abbr `ss8`,Abbr `ss7`,Abbr `ss6`,Abbr `ss5`,Abbr `ss4`,Abbr `ss3`,Abbr `ss2`,
+      Acc_compute_unchanged_state_items,IF_PC_update_unchanged_state_items,
+      ID_pipeline_unchanged_state_items,REG_write_unchanged_state_items,
+      EX_pipeline_unchanged_state_items,MEM_pipeline_unchanged_state_items,
+      WB_pipeline_unchanged_state_items]
+QED
+
+(** data_addr/wstrb/wdata for memory load and store are updated by the agp32_next_state function **)
+Theorem agp32_data_addr_wstrb_wdata_updated_by_agp32_next_state:
+  !fext fbits t s.
+    s = agp32 fext fbits t ==>
+    ((agp32 fext fbits (SUC t)).data_addr = (agp32_next_state (fext t) s s).data_addr) /\
+    ((agp32 fext fbits (SUC t)).data_wstrb = (agp32_next_state (fext t) s s).data_wstrb) /\
+    ((agp32 fext fbits (SUC t)).data_wdata = (agp32_next_state (fext t) s s).data_wdata)
 Proof
   rw [agp32_def,mk_module_def,mk_circuit_def] >>
   qpat_abbrev_tac `s' = mk_circuit (procs _) (procs _) (agp32_init fbits) fext t` >>
